\documentclass[11pt]{scrartcl}
\usepackage[sexy]{../../../evan}
\usepackage{cmbright}
\usepackage{cancel}
\usepackage[T1]{fontenc}
%\usepackage{enumerate}
\usepackage[shortlabels]{enumitem}
\usepackage[utf8]{inputenc}
\usepackage[margin=1in]{geometry}
%\usepackage[pdfborder={0 0 0},colorlinks=true,citecolor=red{}]{hyperref}
\usepackage{amsmath}
\usepackage{amssymb}
\usepackage{setspace}
\usepackage{systeme}

\makeatletter
\newenvironment{Dequation}
{%
	\def\tagform@##1{%
	\maketag@@@{\makebox[0pt][r]{(\ignorespaces##1\unskip\@@italiccorr)}}}%
	\ignorespaces
}
{%
	\def\tagform@##1{\maketag@@@{(\ignorespaces##1\unskip\@@italiccorr)}}%
	\ignorespacesafterend
}
\makeatother

\title{Math 240: Midterm 2 Q5}
\author{Daniel Ko}
\date{Spring 2020}

\begin{document}
\maketitle

\section{Q5}
Consider the following function $f:\{0,1\}^{*} \rightarrow\{0,1\}^{*}$ defined inductively as follows:\\
Foundation rule: $f(\lambda)=\lambda$\\
Constructor rule: $f(x 0)=f(x) 1$ and $f(x 1)=f(x) 0$\\
Prove by structural induction that for all $x \in\{0,1\}^{*}, f(f(x))=x$
\begin{proof}\
	\begin{enumerate}[label=\roman*.]
		\item{
		      Base case: Prove $f(f(\lambda))=\lambda$
		      \begin{align*}
			      f(f(\lambda)) & = f(\lambda) \\
			                    & = \lambda
		      \end{align*}
		      by the foundation rule as desired.
		      }
		\item{
		      Inductive step: Suppose $f(f(n))=n$ where $n \in \{0,1\}^{*}$.
		      We prove that $f(f(ni))=ni$ where $i \in\{0,1\}$. Consider two cases
		      \begin{enumerate}[label=\alph*.]
			      \item{
			            $i = 0$\\\-\\
			            Then, $f(f(ni))=f(f(n0))$
			            \begin{align*}
				            f(f(n0)) & = f(f(n)1) & \text { constructor rule}     \\
				                     & = f(n1)    & \text { inductive hypothesis} \\
				                     & = f(n)0    & \text { constructor rule}     \\
				                     & = n0       & \text { inductive hypothesis}
			            \end{align*}
			            as desired.
			            }
			      \item{
			            $i = 1$\\\-\\
			            Then, $f(f(ni))=f(f(n1))$
			            \begin{align*}
				            f(f(n1)) & = f(f(n)0) & \text { constructor rule}     \\
				                     & = f(n0)    & \text { inductive hypothesis} \\
				                     & = f(n)1    & \text { constructor rule}     \\
				                     & = n1       & \text { inductive hypothesis}
			            \end{align*}
			            as desired.
			            }
		      \end{enumerate}
		      }
	\end{enumerate}
	Therefore, we have proved by structural induction that for all $x \in\{0,1\}^{*}, f(f(x))=x$
\end{proof}
\end{document}
