\documentclass[11pt]{scrartcl}
\usepackage[sexy]{../../evan}
\usepackage{cmbright}
\usepackage{cancel}
\usepackage[T1]{fontenc}
%\usepackage{enumerate}
\usepackage[shortlabels]{enumitem}
\usepackage[utf8]{inputenc}
\usepackage[margin=1in]{geometry}
%\usepackage[pdfborder={0 0 0},colorlinks=true,citecolor=red{}]{hyperref}
\usepackage{amsmath}
\usepackage{amssymb}
\usepackage{setspace}
\usepackage{systeme}

\makeatletter
\newenvironment{Dequation}
  {%
  \def\tagform@##1{%
    \maketag@@@{\makebox[0pt][r]{(\ignorespaces##1\unskip\@@italiccorr)}}}%
  \ignorespaces
  }
  {%
  \def\tagform@##1{\maketag@@@{(\ignorespaces##1\unskip\@@italiccorr)}}%
  \ignorespacesafterend
  }
\makeatother

\title{Math 341: Homework 7}
\author{Daniel Ko}
\date{Spring 2020}

\begin{document}
\maketitle

\section{A}
For each of the following homogeneous systems of linear equations, find the dimension of and a basis for the
solution space.

\begin{enumerate}[label=\alph*.]
	\item{
		\systeme{
			x_1 + 3x_2 = 0,
			2x_1 + 6x_2 = 0
		}
		\begin{proof}
			Using Theorem 3.8 and following example 2 from the textbook, we define this system as an homogeneous system $Ax=0$, where 
			\[
				A=
			\begin{bmatrix}
				1 & 3\\
				2 & 6\\
			\end{bmatrix}\\
			\]
			It is clear that rank(A) = 1 because the two columns are a multiples of each other. 
			If K is	the solution set of this system, then dim(K) = 2 - 1 = 1. 
			Thus any nonzero solution constitutes a basis for K. For example, since
			$
			\begin{pmatrix}
				-3\\
				1\\
			\end{pmatrix}
			$
			is a solution to the given system,
			$
			\begin{Bmatrix}
				\begin{pmatrix}
					-3\\
					1\\
				\end{pmatrix}
			\end{Bmatrix}
			$ 
			is a basis for K by Corollary 2 of Theorem 1.10.
		\end{proof}
	}

	\item{
		\systeme{
			x_1 + 2x_2 - x_3 = 0,
			2x_1 + x_2 + x_3 = 0
		}
		\begin{proof}
			Using Theorem 3.8 and following example 2 from the textbook, we define this system as an homogeneous system $Ax=0$, where 
			\[
				A=
			\begin{bmatrix}
				1 & 2 & -1\\
				2 & 1 & 1\\
			\end{bmatrix}\\
			\]
			It is clear that rank(A) = 2 because there are two linearly independent rows (rank of a transposed matrix is the same as the rank of a matrix).
			If K is	the solution set of this system, then dim(K) = 3 - 2 = 1. 
			Thus any nonzero solution constitutes a basis for K. For example, since
			$
			\begin{pmatrix}
				1\\
				-1\\
				-1\\
			\end{pmatrix}
			$
			is a solution to the given system,
			$
			\begin{Bmatrix}
				\begin{pmatrix}
					1\\
					-1\\
					-1\\
				\end{pmatrix}
			\end{Bmatrix}
			$ 
			is a basis for K by Corollary 2 of Theorem 1.10.
		\end{proof}
	}
	
	\item{
		\systeme{
			x_1 + 2x_2 - 3x_3 + x_4 = 0
		}
		\begin{proof}
			Using Theorem 3.8 and following example 2 from the textbook, we define this system as an homogeneous system $Ax=0$, where 
			\[
				A=
			\begin{bmatrix}
				1 & 2 & -1 & 1\\
			\end{bmatrix}
			\]
			It is clear that rank(A) = 1 because there are one linearly independent row (rank of a transposed matrix is the same as the rank of a matrix).
			If K is	the solution set of this system, then dim(K) = 4 - 1 = 3. 
			Note that, 
			$
			\begin{pmatrix}
				1\\
				1\\
				1\\
				0\\
			\end{pmatrix},
			\begin{pmatrix}
				0\\
				0\\
				1\\
				3\\
			\end{pmatrix},
			\begin{pmatrix}
				1\\
				0\\
				0\\
				-1\\
			\end{pmatrix}
			$
			are linearly independent vectors in K. Thus they form a basis by Corollary 2 of Theorem 1.10.
		\end{proof}
	}
	\item{
		\systeme{
		x_1 + 2x_2 + x_3 + x_4 = 0,
		x_2 - x_3 + x_4 = 0
		}	
		\begin{proof}
			Using Theorem 3.8 and following example 2 from the textbook, we define this system as an homogeneous system $Ax=0$, where 
			\[
				A=
			\begin{bmatrix}
				1 & 2 & 1 & 1\\
				0 & 1 & -1 & 1\\
			\end{bmatrix}
			\]
			It is clear that rank(A) = 2 because there are 2 linearly independent rows (rank of a transposed matrix is the same as the rank of a matrix).
			If K is	the solution set of this system, then dim(K) = 4 - 2 = 2. 
			Note that, 
			$
			\begin{pmatrix}
				2\\
				0\\
				-1\\
				-1\\
			\end{pmatrix},
			\begin{pmatrix}
				-4\\
				2\\
				1\\
				-1\\
			\end{pmatrix}
			$
			are linearly independent vectors in K. Thus they form a basis by Corollary 2 of Theorem 1.10.
		\end{proof}
	}
	\item{
		\systeme{
			x_1 + x_2 - x_3 = 0,
			4x_1 + x_2 - 2x_3 = 0
			}	
		\begin{proof}
			Using Theorem 3.8 and following example 2 from the textbook, we define this system as an homogeneous system $Ax=0$, where 
			\[
				A=
			\begin{bmatrix}
				1 & 1 & -1\\
				4 & 1 & -2\\
			\end{bmatrix}
			\]
			It is clear that rank(A) = 2 because there are 2 linearly independent rows (rank of a transposed matrix is the same as the rank of a matrix).
			If K is	the solution set of this system, then dim(K) = 3 - 2 = 1. 
			Thus any nonzero solution constitutes a basis for K. For example, since
			$
			\begin{pmatrix}
				1\\
				2\\
				3\\
			\end{pmatrix}
			$
			is a solution for K, it forms a basis by Corollary 2 of Theorem 1.10.
		\end{proof}
		}
	\item{
		\systeme{
			2x_1 + x_2 - x_3 = 0,
			x_1 - x_2 + x_3 = 0,
			x_1 + 2x_2 - 2x_3 = 0
		}
		\begin{proof}
			Using Theorem 3.8 and following example 2 from the textbook, we define this system as an homogeneous system $Ax=0$, where 
			\[
				A=
			\begin{bmatrix}
				2 & 1 & -1\\
				1 & -1 & 1\\
				1 & 2 & -2\\
			\end{bmatrix}
			\]
			It is clear that rank(A) = 2 because there are 2 linearly independent columns (third column is second column multiplied by -1).
			If K is	the solution set of this system, then dim(K) = 3 - 2 = 1. 
			Thus any nonzero solution constitutes a basis for K. For example, since
			$
			\begin{pmatrix}
				0\\
				1\\
				1\\
			\end{pmatrix}
			$
			is a solution for K, it forms a basis by Corollary 2 of Theorem 1.10.
		\end{proof}
	}
	\item{
	\systeme{
		x_1 + 2x_2 = 0,
		x_1 - x_2 = 0
		}
	\begin{proof}
		Using Theorem 3.8 and following example 2 from the textbook, we define this system as an homogeneous system $Ax=0$, where 
		\[
			A=
		\begin{bmatrix}
			1 & 2\\
			1 & -1\\
		\end{bmatrix}
		\]
		It is clear that rank(A) = 2 because there are 2 linearly independent columns.
		If K is	the solution set of this system, then dim(K) = 2 - 2 = 0. 
		This means the zero vector is the basis for K, i.e.
		$
		\begin{pmatrix}
			0\\
			0\\
		\end{pmatrix}
		$.
	\end{proof}
	}
\end{enumerate}

\section{B}
Using the results of Exercise 2, find all solutions to the following systems.
\begin{enumerate}[label=\alph*.]

	\item{
		\systeme{
			x_1 + 3x_2 = 5,
			2x_1 + 6x_2 = 10
		}
		\begin{proof}
			A solution to the above system is  
			$
			\begin{pmatrix}
				2\\
				1\\
			\end{pmatrix}
			$.
			Using Theorem 3.9 and following example 3 from the textbook, we know $K = \{s\} + K_H = \{s + k : k \in K_H \}$.
			So, 
			\[
			K=
			\left\{
				\begin{pmatrix}
					2\\
					1\\
				\end{pmatrix}
				+ 
				t\begin{pmatrix}
					-3\\
					1\\
				\end{pmatrix}: t \in \mathbb{R}
			\right\}
			\]
		\end{proof}
	}
	
	\item{
		\systeme{
			x_1 + 2x_2 - x_3 = 3,
			2x_1 + x_2 + x_3 = 6
		}
		\begin{proof}
			A solution to the above system is  
			$
			\begin{pmatrix}
				1\\
				2\\
				2\\
			\end{pmatrix}
			$.
			Using Theorem 3.9 and following example 3 from the textbook, we know $K = \{s\} + K_H = \{s + k : k \in K_H \}$.
			So, 
			\[
			K=
			\left\{
				\begin{pmatrix}
					1\\
					2\\
					2\\
				\end{pmatrix}
				+ 
				t\begin{pmatrix}
					1\\
					-1\\
					-1\\
				\end{pmatrix}: t \in \mathbb{R}
			\right\}
			\]
		\end{proof}
	}
	\item{
		\systeme{
			x_1 + 2x_2 - 3x_3 + x_4 = 1
		}
		\begin{proof}
			A solution to the above system is  
			$
			\begin{pmatrix}
				1\\
				0\\
				0\\
				0\\
			\end{pmatrix}
			$.	
			Using Theorem 3.9 and following example 3 from the textbook, we know $K = \{s\} + K_H = \{s + k : k \in K_H \}$.
			So, 
			\[
			K=
			\left\{
				\begin{pmatrix}
					1\\
					0\\
					0\\
					0\\
				\end{pmatrix} +
				t_1\begin{pmatrix}
					1\\
					1\\
					1\\
					0\\
				\end{pmatrix}+
				t_2\begin{pmatrix}
					0\\
					0\\
					1\\
					3\\
				\end{pmatrix}+
				t_3\begin{pmatrix}
					1\\
					0\\
					0\\
					-1\\
				\end{pmatrix}: t_1, t_2, t_3 \in \mathbb{R}
			\right\}
			\]
		\end{proof}
		}

	\item{ 
		\systeme{
			x_1 + 2x_2 + x_3 + x_4 = 1,
			x_2 - x_3 + x_4 = 1	
		}	
		\begin{proof}
			A solution to the above system is  
			$
			\begin{pmatrix}
				0\\
				0\\
				0\\
				1\\
			\end{pmatrix}
			$.	
			Using Theorem 3.9 and following example 3 from the textbook, we know $K = \{s\} + K_H = \{s + k : k \in K_H \}$.
			So, 
			\[
			K=
			\left\{
				\begin{pmatrix}
					0\\
					0\\
					0\\
					1\\
				\end{pmatrix} +
				t_1\begin{pmatrix}
					2\\
					0\\
					-1\\
					-1\\
				\end{pmatrix}+
				t_2\begin{pmatrix}
					-4\\
					2\\
					1\\
					-1\\
				\end{pmatrix}: t_1, t_2 \in \mathbb{R}
			\right\}
			\]
		\end{proof}
	}
	\item{
		\systeme{
			x_1 + x_2 - x_3 = 1,
			4x_1 + x_2 - 2x_3 = 3
			}	
		\begin{proof}
			A solution to the above system is  
			$
			\begin{pmatrix}
				1\\
				1\\
				1\\
			\end{pmatrix}
			$.	
			Using Theorem 3.9 and following example 3 from the textbook, we know $K = \{s\} + K_H = \{s + k : k \in K_H \}$.
			So, 
			\[
			K=
			\left\{
				\begin{pmatrix}
					1\\
					1\\
					1\\
				\end{pmatrix} +
				t\begin{pmatrix}
					1\\
					2\\
					3\\
				\end{pmatrix}: t \in \mathbb{R}
			\right\}
			\]
		\end{proof}
	}
	\item{
		\systeme{
			2x_1 + x_2 - x_3 = 5,
			x_1 - x_2 + x_3 = 1,
			x_1 + 2x_2 - 2x_3 = 4
		}
		\begin{proof}
			A solution to the above system is  
			$
			\begin{pmatrix}
				2\\
				1\\
				0\\
			\end{pmatrix}
			$.	
			Using Theorem 3.9 and following example 3 from the textbook, we know $K = \{s\} + K_H = \{s + k : k \in K_H \}$.
			So, 
			\[
			K=
			\left\{
				\begin{pmatrix}
					2\\
					1\\
					0\\
				\end{pmatrix} +
				t\begin{pmatrix}
					0\\
					1\\
					1\\
				\end{pmatrix}: t \in \mathbb{R}
			\right\}
			\]
		\end{proof}
	}
	\item{
		\systeme{
			x_1 + 2x_2 = 5,
			x_1 - x_2 = -1
			}
		\begin{proof}
			A solution to the above system is  
			$
			\begin{pmatrix}
				1\\
				2\\
			\end{pmatrix}
			$.	
			Using Theorem 3.9 and following example 3 from the textbook, we know $K = \{s\} + K_H = \{s + k : k \in K_H \}$.
			So, 
			\[
			K=
			\left\{
				\begin{pmatrix}
					1\\
					2\\
				\end{pmatrix} +
				t\begin{pmatrix}
					0\\
					0\\
				\end{pmatrix}: t \in \mathbb{R}
			\right\} = 
			\left\{
				\begin{pmatrix}
					1\\
					2\\
				\end{pmatrix} 
			\right\}
			\]
		\end{proof}	
	}
\end{enumerate}

\section{C}
Prove that the system of linear equations $Ax = b$ has a solution if and only if $b \in R(L_A)$.
\begin{proof}
	Let $A$ be an $mxn$ matrix.
	\begin{enumerate}[i.]
		\item{
			$Ax = b$ has a solution $\Rightarrow b \in R(L_A)$.\\\-\\
			Let $s$ be a solution to $Ax = b$. This means $A_1s_1 + \cdots + A_ns_n = b$. 
			Notice that $b$ is a linear combination of the columns of $A$, 
			which is equivalent to $R(L_A)$ by the proof given in Theorem 3.5. 
			Therefore, $b \in R(L_A)$.
		}
		\item{
			$b \in R(L_A) \Rightarrow Ax = b$ has a solution.\\\-\\
			$b \in R(L_A)$ means that $b$ is a linear combination of the columns of $A$. 
			So, $b = A_1s_1 + \cdots + A_ns_n$. 
			This means there exists an $x$, composed of the $s_1, \cdots, s_n$ as seen in the previous equation, such that $Ax = b$.  
			Therfore, $Ax = b$ has a solution.
		}
	\end{enumerate}
\end{proof}

\section{D}
Prove or give a counterexample to the following statement: If the comatrix of a system of $m$ linear equations in
$n$ unknowns has rank $m$, then the system has a solution.
\begin{proof}
Let $A$ be a $mxn$ comatrix for the system $Ax=b$. By defintion, $L_A: \mathbb{F}^n \rightarrow \mathbb{F}^m$. 
Another way of saying that the system has a solution is to say that $b \in R(L_A)$, as we proved
in problem C. Given that the rank$(A)=m$, it follows that that dim$(R(L_A)) = m $ by Theorem 3.5. 
Since the range and the codomain of $L_A$ are the same, it means that $L_A$ is onto by definition. 
Thus, $\forall b \in R(L_A) [\exists s \in \mathbb{F}^n \text{ s.t. } As = b]$.
Therefore, if the comatrix of a system of $m$ linear equations in
$n$ unknowns has rank $m$, then system has a solution.
\end{proof}
	

\section{E}
Suppose that the augmented matrix of a system $Ax = b$ is transformed into a matrix $(A'|b')$ in reduced row
echelon form by a finite sequence of elementary row operations.
\begin{enumerate}[label=\alph*.]
	\item{
		Prove that rank($A'$), rank$(A'|b')$ if and only if $(A'|b')$ contains a row in which the only nonzero entry lies
		in the last column.

	}
	\item{
		Deduce that $Ax = b$ is consistent if and only if $(A'|b')$ contains no row in which the only nonzero entry lies
		in the last column.
	}
\end{enumerate}


\section{F}

\section{G}

\section{H} 

\section{I} 
Prove the corollary to Theorem 3.16: The reduced row echelon form of a matrix is unique.
\begin{proof}
Let's assume for the sake of contradiction that matrix $A$ has two unique reduced row echelon forms, $B$ and $B'$.
Theorem 3.16(b) states that "For each $k = 1, 2, \cdots, n$, if column $k$ of $B$ is $d_1e_1 + d_2e_2 + \cdots + d_re_r $, 
then column $k$ of $A$ is $d_1a_{j_1} + d_2a_{j_2} + \cdots + d_ra_{j_r}$. Let's the $k$ column of $B$ be $d_1e_1 + d_2e_2 + \cdots + d_re_r$
and the $k$ column of $B'$ be $d'_1e_1 + d'_2e_2 + \cdots + d'_re_r$ where $kth$ column of $B$ does not equal the $kth$ column of $B'$ because they are both unique.
However, this would be that the $k$th column of the original matrix $A$ are different depending if you compute using $B$ or $B'$. Thus, this is a contradiction
and $A$ must have a unique reduced row echelon form. 
\end{proof}
\end{document}